Divergence.v
@@ -1,0 +1,166 @@
+From Coq Require Import Program.Equality.
+From Coinduction Require Import all.
+From RelationAlgebra Require Import
+     kat
+     kat_tac
+     prop
+     rel
+     srel
+     comparisons
+     rewriting
+     normalisation
+     monoid.
+From OptSim Require Import Utils LTS.
+
+Import CoindNotations.
+
+Section WithLTS.
+
+Context {lts : LTS}.
+Let Observable := lts.(Observable).
+Let St := lts.(St).
+Let trans := lts.(trans).
+Let epsilon := lts.(epsilon).
+Let Robs := lts.(Robs).
+Let ub_state := lts.(ub_state).
+Let label := @label Observable.
+
+Program Definition divergesF : mon (St -> Prop) :=
+{| body R st :=
+  exists st', trans tau st st' /\ R st'
+|}.
+Next Obligation.
+  eauto.
+Qed.
+
+Definition diverges := gfp divergesF.
+
+#[export] Instance : Proper (St.(Eq) ==> impl) diverges.
+Proof.
+  cbn. red. coinduction R CH. intros.
+  apply (gfp_fp divergesF) in H0. destruct H0 as (? & ? & ?).
+  rewrite H in H0. exists x0. eauto.
+Qed.
+
+Variant DTauAnswer (R Rind : relation St) s' t : Prop :=
+| dtau_match t' (TR : trans tau t t') (DIV : R s' t')
+| dtau_div (DIV : Rind s' t)
+.
+Hint Resolve dtau_match 2 : optsim.
+Hint Resolve dtau_div 3 : optsim.
+
+#[export] Instance DTauAnswer_eq R Rind :
+  Proper (Eq St ==> Eq St ==> impl) R ->
+  Proper (Eq St ==> Eq St ==> impl) Rind ->
+  Proper (Eq St ==> Eq St ==> impl) (DTauAnswer R Rind).
+Proof.
+  intros. cbn. intros. destruct H3.
+  - rewrite H2 in TR. rewrite H1 in DIV. esim.
+  - rewrite H1, H2 in DIV. esim.
+Qed.
+
+Definition divpresIndF R Rind s t :=
+  forall s', trans tau s s' -> DTauAnswer R Rind s' t.
+Hint Unfold divpresIndF : optsim.
+
+Section NoElim.
+#[local] Unset Elimination Schemes.
+Inductive divpresInd R s t : Prop :=
+| divpresI : divpresIndF R (divpresInd R) s t -> divpresInd R s t.
+End NoElim.
+Hint Constructors divpresInd : optsim.
+
+Definition divpresInd_ind :
+  forall R P : St -> St -> Prop,
+       (forall s t : St,
+         (divpresIndF R (fun s t => divpresInd R s t /\ P s t) s t) -> 
+        P s t) -> forall t t0 : St, divpresInd R t t0 -> P t t0.
+Proof.
+  intros until 1. fix F 3. intros. apply H. destruct H0.
+  red. intros. apply H0 in H1 as [].
+  - eleft; eauto.
+  - eright; eauto.
+Qed.
+
+Program Definition divpresF : mon (St -> St -> Prop) :=
+{| body R s t := divpresInd R s t |}.
+Next Obligation.
+  induction H0. constructor. intros ??.
+  apply H0 in H1 as []. eleft; eauto. eright; eauto. apply DIV.
+Qed.
+
+Lemma unfold_divpresF : forall R s t,
+ divpresInd R s t ->
+ divpresF R s t.
+Proof.
+  auto.
+Qed.
+Hint Resolve unfold_divpresF : optsim.
+
+#[export] Instance divpresF_eq R :
+  Proper (Eq St ==> Eq St ==> impl) R ->
+  Proper (Eq St ==> Eq St ==> impl) (divpresF R).
+Proof.
+  intro. cbn. intros.
+  revert y y0 H0 H1. induction H2. intros. constructor. intros ??.
+  rewrite <- H1 in H3.
+  apply H0 in H3 as [].
+  - rewrite H2 in TR. esim.
+  - right. now eapply DIV.
+Qed.
+
+Inductive nodiv s : Prop :=
+| nodiv_tau : (forall s', trans tau s s' -> nodiv s') -> nodiv s
+.
+
+Lemma diverges_nodiv : forall s,
+  nodiv s ->
+  diverges s ->
+  False.
+Proof.
+  intros. induction H.
+  apply (gfp_fp divergesF) in H0 as (? & ? & ?).
+  apply H1 in H0 as [].
+  apply H2.
+Qed.
+
+Lemma diverges_impl_nodiv : forall (s t : St),
+  nodiv s \/ diverges t ->
+  (diverges s -> diverges t).
+Proof.
+  intros. destruct H.
+  - now apply diverges_nodiv in H; auto.
+  - apply H.
+Qed.
+
+Definition divpres := gfp divpresF.
+
+Axiom diverges_lem : forall s, diverges s \/ nodiv s.
+
+Lemma divpres_impl : forall s t,
+  divpres s t ->
+  diverges s -> diverges t.
+Proof.
+  red. coinduction R CH. intros.
+  apply (gfp_fp divpresF) in H. induction H. apply (gfp_fp divergesF) in H0 as (? & ? & ?).
+  apply H in H0 as [].
+  - exists t'. eauto.
+  - now apply DIV.
+Qed.
+
+Lemma diverges_divpres :
+  forall s t, diverges t -> divpres s t.
+Proof.
+  red. coinduction R CH.
+  intros. constructor. intros ??.
+  apply (gfp_fp divergesF) in H as (? & ? & ?).
+  eleft; eauto.
+Qed.
+
+End WithLTS.
+
+Hint Resolve dtau_match 2 : optsim.
+Hint Resolve dtau_div 3 : optsim.
+Hint Unfold divpresIndF : optsim.
+Hint Constructors divpresInd : optsim.
+Hint Resolve unfold_divpresF : optsim.
