IndSim.v
@@ -1,0 +1,74 @@
+From RelationAlgebra Require Import
+     kat
+     kat_tac
+     prop
+     rel
+     srel
+     comparisons
+     rewriting
+     normalisation
+     monoid.
+From Coinduction Require Import all.
+From OptSim Require Import Utils LTS OptSim.
+
+Section WithLTS.
+
+Context {lts : LTS}.
+Context (freeze : SimOpt.freeze_opt) (lock : SimOpt.lock_opt) (delay : SimOpt.delay_opt).
+Let Observable := lts.(Observable).
+Let St := lts.(St).
+Let trans := lts.(trans).
+Let epsilon := lts.(epsilon).
+Let Robs := lts.(Robs).
+Let ub_state := lts.(ub_state).
+Let label := @label Observable.
+
+  Variant TauIndAnswer (R Rind : relation St) s' t : Prop :=
+  | taui_exact t' (TR : trans tau t t') (SIM : R s' t')
+  | taui_freeze (_ : freeze = SimOpt.freeze) (SIM : R s' t)
+  | taui_div (_ : freeze = SimOpt.freeze_div) (SIM : Rind s' t)
+  | taui_delay t' (_ : delay = SimOpt.delay) (TR : (trans tau)^+ t t') (SIM : R s' t')
+  .
+  Hint Constructors TauIndAnswer : optsim.
+
+  Definition simIndF R Rind s t :=
+    (forall o s', trans (obs o) s s' ->
+      ObsAnswer delay R s' t o
+    ) /\
+    (forall s', trans tau s s' ->
+      TauIndAnswer R Rind s' t
+    ) /\
+    (lock = SimOpt.nolock \/ (is_stuck s -> is_stuck t)).
+
+  Section NoElim.
+  #[local] Unset Elimination Schemes.
+  Inductive simInd R s t : Prop :=
+  | simI :
+    simIndF R (simInd R) s t -> simInd R s t.
+  End NoElim.
+
+  Definition simInd_ind :
+    forall R P : St -> St -> Prop,
+         (forall s t : St,
+           (simIndF R (fun s t => simInd R s t /\ P s t) s t) -> 
+          P s t) -> forall t t0 : St, simInd R t t0 -> P t t0.
+  Proof.
+    intros until 1. fix F 3. intros. apply H. destruct H0. repeat split; intros.
+    - apply H0 in H1 as [].
+      eleft; eauto.
+      eright; eauto.
+    - apply H0 in H1 as []; esim.
+    - apply H0.
+  Qed.
+
+Lemma simInd_mon : forall R R', R <= R' -> simInd R <= simInd R'.
+Proof.
+  cbn. intros. induction H0.
+  repeat split; intros.
+  - apply H0 in H1 as []; esim.
+  - apply H0 in H1 as []; esim.
+    destruct SIM. esim.
+  - apply H0.
+Qed.
+
+End WithLTS.
