LTS.v
@@ -1,0 +1,91 @@
+From Coq Require Import Morphisms.
+From RelationAlgebra Require Import srel lattice rel.
+
+Variant label {S : Type} := obs (s : S) | tau.
+
+Record LTS := {
+  Observable : Type;
+  St : EqType;
+  trans : @label Observable -> srel St St;
+  epsilon : srel St St;
+  Robs : Observable -> Observable -> Prop;
+  ub_state : St -> Prop;
+}.
+
+Arguments trans {lts} : rename.
+Arguments epsilon {lts} : rename.
+Arguments Robs {lts} : rename.
+Arguments ub_state {lts} : rename.
+
+(*Section LockLTS.
+
+  Context (lts : LTS).
+  Variant LockObservable := | Event (e : lts.(Observable)) | NoEvent.
+  Program Definition LockSt := {| type_of := (bool * lts.(St))%type |}.
+  Variant locktrans : @label LockObservable -> LockSt -> LockSt -> Prop :=
+  | locktrans_ev b o s t : lts.(trans) (obs o) s t -> locktrans (obs (Event o)) (b, s) (true, t)
+  | locktrans_noev s : (forall l t, lts.(trans) l s t -> False) -> locktrans (obs NoEvent) (true, s) (true, s)
+  .
+  Definition lockepsilon : LockSt -> LockSt -> Prop :=
+    fun '(b, s) '(b', s') =>
+    lts.(epsilon) s s' /\ (
+      (b = false /\ b' = false) \/
+      (b = true /\ b' = false) \/
+      (b = true /\ b' = true /\ forall l s'', lts.(trans) l s s'' -> False)
+    ).
+  Definition LockRobs : LockObservable -> LockObservable -> Prop. Admitted.
+  Definition lock_ub_state : LockSt -> Prop. Admitted.
+
+  Definition lock := {|
+    Observable := LockObservable;
+    St := LockSt;
+    trans := locktrans;
+    epsilon := lockepsilon;
+    Robs := LockRobs;
+    ub_state := lock_ub_state
+  |}.
+
+End LockLTS.*)
+
+Section LTS.
+
+Context {lts : LTS}.
+
+#[global] Instance :
+  Proper (weq ==> eq ==> eq ==> iff) (hrel_of (n := lts.(St)) (m := lts.(St))).
+Proof.
+  cbn. intros. subst. apply H.
+Qed.
+
+#[global] Instance : Proper (leq ==> eq ==> eq ==> impl) (hrel_of (n := lts.(St)) (m := lts.(St))).
+Proof.
+  cbn. intros. subst. now apply H.
+Qed.
+
+Definition is_obs (l : @label lts.(Observable)) := if l then true else false.
+Definition is_tau (l : @label lts.(Observable)) := if l then false else true.
+
+Definition is_tau_state st :=
+  forall l st', lts.(trans) l st st' -> is_tau l = true.
+
+Definition is_obs_state st :=
+  forall l st', lts.(trans) l st st' -> is_obs l = true.
+
+Variant extrans (st : lts.(St)) : Prop :=
+  trans_intro l st' : trans l st st' -> extrans st.
+Hint Constructors extrans : optsim.
+
+#[export] Instance : Proper (lts.(St).(Eq) ==> flip impl) extrans.
+Proof.
+  cbn. intros ??? []. rewrite <- H in H0. eauto with optsim.
+Qed.
+
+Definition is_stuck (st : lts.(St)) : Prop :=
+  ~ extrans st.
+
+#[export] Instance : Proper (lts.(St).(Eq) ==> flip impl) is_stuck.
+Proof.
+  cbn. unfold is_stuck. intros. now setoid_rewrite H.
+Qed.
+
+End LTS.
