Utils.v
@@ -1,0 +1,82 @@
+From RelationAlgebra Require Import
+     kat
+     kat_tac
+     prop
+     rel
+     srel
+     comparisons
+     rewriting
+     normalisation
+     monoid.
+
+Create HintDb optsim.
+#[global] Ltac esim := eauto 10 with optsim exfalso.
+
+(* RA lemmas *)
+
+Lemma itr_unfold_l `{laws} `{KA ≪ l} :
+  forall (n : ob X) (x : X n n), x^+ ≡ x + x⋅x^+.
+Proof.
+  intros. now rewrite itr_str_l, str_unfold_l, <- itr_str_l, dotxpls, dotx1 at 1.
+Qed.
+
+Lemma itr_unfold_r `{laws} `{KA ≪ l} :
+  forall (n : ob X) (x : X n n), x^+ ≡ x + x^+⋅x.
+Proof.
+  intros. now rewrite itr_str_r, kleene.str_unfold_r, <- itr_str_r, dotplsx, dot1x at 1.
+Qed.
+
+Lemma str_itr' `{laws} `{KA ≪ l} :
+  forall (n : ob X) (x : X n n), x^+ ≦ x^*.
+Proof.
+  intros. now rewrite str_itr, <- leq_cup_r.
+Qed.
+
+Lemma srel_str_ind_l {E : EqType} :
+  forall (P : E -> Prop) (i : srel E E),
+  Proper (E.(Eq) ==> iff) P ->
+  (forall s t : E, i s t -> P t -> P s) ->
+  forall s t : E, i^* s t -> P t -> P s.
+Proof.
+  intros.
+  eset (P' := {| hrel_of := fun s t => P t -> P s|} : srel E E).
+  epose proof (str_ind_l1 (X := srel_monoid_ops)). specialize (H3 E i P'). cbn in H3. eapply H3.
+  - intros. now rewrite H4.
+  - intros. red in H4. destruct H4. eauto.
+  - apply H1.
+  - apply H2.
+  Unshelve.
+  cbn. intros. now rewrite H3, H4.
+Qed.
+
+Lemma srel_str_ind_r {E : EqType} :
+  forall (P : E -> Prop) (i : srel E E),
+  Proper (E.(Eq) ==> iff) P ->
+  (forall s t : E, i s t -> P s -> P t) ->
+  forall s t : E, i^* s t -> P s -> P t.
+Proof.
+  intros.
+  eset (P' := {| hrel_of := fun s t => P s -> P t|} : srel E E).
+  epose proof (str_ind_r1 (X := srel_monoid_ops)). specialize (H3 E i P'). cbn in H3. eapply H3.
+  - intros. now rewrite <- H4.
+  - intros. red in H4. destruct H4. eapply H0; eauto.
+  - apply H1.
+  - apply H2.
+  Unshelve.
+  cbn. intros. now rewrite H3, H4.
+Qed.
+
+Lemma srel_str_ind_l' {E : EqType} :
+  forall (i : srel E E) (P : E -> E -> Prop),
+  Proper (E.(Eq) ==> E.(Eq) ==> iff) P ->
+  (forall s t, E.(Eq) s t -> P s t) ->
+  (forall s t u, i s t -> P t u -> P s u) ->
+  forall s t, i^* s t -> P s t.
+Proof.
+  intros.
+  eset (P' := {| hrel_of := fun s t => P s t|} : srel E E).
+  epose proof (str_ind_l1 (X := srel_monoid_ops)). specialize (H3 E i P'). cbn in H3. eapply H3.
+  - intros. now apply H0.
+  - intros. red in H4. destruct H4. eapply H1; eauto.
+  - apply H2.
+Qed.
